---
title: "chapter4"
author: "Nikunj Goel"
date: "10/12/2020"
output: html_document
---

```{r setup, include=FALSE}
knitr::opts_chunk$set(echo = TRUE)
```

## Problem 4.2

### Part a)

Using **Mathematical Induction** to prove the formula
$$
x_{t} = \sum_{j=0}^{t}\phi^jw_{t-j}
\\
x_{0} = w_{0}
\\
x_{1} = \phi^0w_{1} + \phi^1w_{0}
\\
x_{2} = \phi^0w_{2} + \phi^1w_{1} +\phi^2w_{0}
\\
x_{3} = \phi^0w_{3} + \phi^1w_{2} +\phi^2w_{1} + \phi^3w_{0}
\\
Assuming \ it \ to \ be \ true \ for \ x_{t-1}
\\
The \ expression \ hold \ for \ x_{t} 
\\
x_{t} = \phi(\sum_{k=0}^\infty \phi^kw_{t-1-k}) + w_{t}
\\
Hence \ Proved
$$
### Part b)

$$
Right \  hand \ side \ is
\\
= w_{t} + \phi w_{t-1}[k=0] + \phi^2w_{t-2}[k=1] + ...
\\
E(x_{t}) = \sum_{j=0}^{\infty}\phi^jE(w_{t-j}) = 0
$$
 